compiler/src/compiler/ExprImpEventLoopSpec.v
@@ -40,12 +40,12 @@ Section Params1.
     get_init_code: map.get (map.of_list e) init_f = Some (nil, nil, init_code);
     init_code_correct: forall m0 mc0,
         mem_available spec.(datamem_start) spec.(datamem_pastend) m0 ->
-        Semantics.exec (map.of_list e) init_code nil m0 map.empty mc0 (hl_inv spec);
+        MetricSemantics.exec (map.of_list e) init_code nil m0 map.empty mc0 (hl_inv spec);
     loop_body: Syntax.cmd.cmd;
     get_loop_body: map.get (map.of_list e) loop_f = Some (nil, nil, loop_body);
     loop_body_correct: forall t m l mc,
         hl_inv spec t m l mc ->
-        Semantics.exec (map.of_list e) loop_body t m l mc (hl_inv spec);
+        MetricSemantics.exec (map.of_list e) loop_body t m l mc (hl_inv spec);
   }.
 
 End Params1.
